---
sidebar_position: 030_020
---

# Surds

A **surd** is an expression that includes a root, such as a square root or cube
root. Surds are often used to represent irrational numbers.

## Simplifying surds

- To simplify a surd, we need to look for any factors that are **squares**.
- We can then take the square root of these factors out of the surd.

### Example: simplify $\sqrt{48}$

- $=\sqrt{16\times3}$
- $=\sqrt{16}\times\sqrt{3}$
- $=4\sqrt{3}$

### Example: simplify $\sqrt{18}$

- $=\sqrt{9\times2}$
- $=\sqrt{9}\times\sqrt{2}$
- $=3\sqrt{2}$

### Example: simplify $\sqrt{50}$

- $=\sqrt{25\times2}$
- $=\sqrt{25}\times\sqrt{2}$
- $=5\sqrt{2}$

## Adding surds

We can only add surds that have the same **surd part** (the part under the
root).

When adding surds with the same surd part, we simply add the coefficients (the
numbers in front of the surd).

### Example: simplify $3\sqrt{2}+5\sqrt{2}$

- $=(3+5)\sqrt{2}$
- $=8\sqrt{2}$

### Example: simplify $7\sqrt{3}-2\sqrt{3}$

- $=(7-2)\sqrt{3}$
- $=5\sqrt{3}$

## Subtracting surds

We can only subtract surds that have the same **surd part** (the part under the
root).

When subtracting surds with the same surd part, we simply subtract the
coefficients (the numbers in front of the surd).

### Example: simplify $6\sqrt{5}-4\sqrt{5}$

- $=(6-4)\sqrt{5}$
- $=2\sqrt{5}$

### Example: simplify $9\sqrt{7}-3\sqrt{7}$

- $=(9-3)\sqrt{7}$
- $=6\sqrt{7}$

## Multiplying surds

When multiplying surds, we can multiply the numbers outside the surds and the
numbers inside the surds separately.

This can be written as:

$$
a\sqrt{x}\times b\sqrt{y}=(a\times b)\sqrt{xy}
$$

### Example: simplify $2\sqrt{3}\times4\sqrt{5}$

- $=(2\times4)\sqrt{3\times5}$
- $=8\sqrt{15}$

### Example: simplify $3\sqrt{2}\times5\sqrt{6}$

- $=(3\times5)\sqrt{2\times6}$
- $=15\sqrt{12}$
- $=15\sqrt{4\times3}$
- $=15\times2\sqrt{3}$
- $=30\sqrt{3}$

## Dividing surds

When dividing surds, we can divide the numbers outside the surds and the
numbers inside the surds separately.

This can be written as:

$$
\frac{a\sqrt{x}}{b\sqrt{y}}=\frac{a}{b}\sqrt{\frac{x}{y}}
$$

### Example: simplify $\frac{6\sqrt{8}}{3\sqrt{2}}$

- $=\frac{6}{3}\sqrt{\frac{8}{2}}$
- $=2\sqrt{4}$
- $=2\times2$
- $=4$

### Example: simplify $\frac{10\sqrt{18}}{5\sqrt{2}}$

- $=\frac{10}{5}\sqrt{\frac{18}{2}}$
- $=2\sqrt{9}$
- $=2\times3$
- $=6$

## Rationalising the denominator

When we have a surd in the denominator of a fraction, we can **rationalise** the
denominator by multiplying both the numerator and denominator by the surd (or
the negated factor).

### Example: rationalise $\frac{1}{\sqrt{2}}$

- $=\frac{1\times\sqrt{2}}{\sqrt{2}\times\sqrt{2}}$
- $=\frac{\sqrt{2}}{2}$

### Example: rationalise $\frac{3}{\sqrt{5}}$

- $=\frac{3\times\sqrt{5}}{\sqrt{5}\times\sqrt{5}}$
- $=\frac{3\sqrt{5}}{5}$

### Example: rationalise $\frac{4}{\sqrt{3}}$

- $=\frac{4\times\sqrt{3}}{\sqrt{3}\times\sqrt{3}}$
- $=\frac{4\sqrt{3}}{3}$

### Example: rationalise $\frac{\sqrt{2}}{1+\sqrt{3}}$

- $=\frac{\sqrt{2}(1-\sqrt{3})}{(1+\sqrt{3})(1-\sqrt{3})}$
- $=\frac{\sqrt{2}-\sqrt{6}}{1-3}$
- $=\frac{\sqrt{2}-\sqrt{6}}{-2}$

### Example: rationalise $\frac{5}{2+\sqrt{7}}$

- $=\frac{5(2-\sqrt{7})}{(2+\sqrt{7})(2-\sqrt{7})}$
- $=\frac{10-5\sqrt{7}}{4-7}$
- $=\frac{10-5\sqrt{7}}{-3}$

### Example: rationalise $\frac{3\sqrt{5}}{4-\sqrt{2}}$

- $=\frac{3\sqrt{5}(4+\sqrt{2})}{(4-\sqrt{2})(4+\sqrt{2})}$
- $=\frac{12\sqrt{5}+3\sqrt{10}}{16-2}$
- $=\frac{12\sqrt{5}+3\sqrt{10}}{14}$

