---
title: Changing the base of a power
---

We know from the page on [raising an index to an index](/raising-an-index-to-an-index)
that we can rewrite $(a^x)^y$ as $a^{xy}$.

<!--Similarly, we can go the other way. If we know that the factors of the index are
multiplying together to give the index, we can rewrite the power as a power of a
power: $a^{xy} = (a^x)^y$.-->

### Example: write $2^6$ as a power of $2^2$

- $=2^{2\times3}$
- $=(2^2)^3$

### Example: write $81^3$ as a power of $3$

We can rewrite $81$ as $3^4$, so:
- $81^3$
- $=(3^4)^3$
- $=3^{4\times3}$
- $=3^{12}$

### Example: write $16^4$ as a power of $2$

We can rewrite $16$ as $2^4$, so:
- $16^4$
- $=(2^4)^4$
- $=2^{4\times4}$
- $=2^{16}$

### Example: write $27^5$ as a power of $3$

We can rewrite $27$ as $3^3$, so:
- $27^5$
- $=(3^3)^5$
- $=3^{3\times5}$
- $=3^{15}$

### Example: write $64^2$ as a power of $4$

We can rewrite $64$ as $4^3$, so:
- $64^2$
- $=(4^3)^2$
- $=4^{3\times2}$
- $=4^{6}$

