---
title: Converting logarithms into exponentials
---

We can also convert logarithmic expressions into exponential ones using the
same exact definition of logarithms:

$$
\log_a(b) = c \quad \text{is equivalent to} \quad a^c = b
$$

### Convert $\log_2(8)=3$ into an exponential expression

- $\log_a(b) = c$ is equivalent to $a^c = b$
- $a=2$, $b=8$, and $c=3$
- $2^3=8$

### Convert $\log_5(25)=2$ into an exponential expression

- $\log_a(b) = c$ is equivalent to $a^c = b$
- $5^2=25$

### Convert $\log_3(27)=3$ into an exponential expression

- $\log_a(b) = c$ is equivalent to $a^c = b$
- $3^3=27$

### Write as an exponential expression: $\log_{10}(1000)=x$

- $\log_a(b) = c$ is equivalent to $a^c = b$
- $10^x=1000$

### Write as an exponential expression: $\ln(7)=x$

- $\ln(7)=\log_e(7)$
- $\log_a(b) = c$ is equivalent to $a^c = b$
- $e^x=7$

### Write as an exponential expression: $\log_4(x)=2$

- $\log_a(b) = c$ is equivalent to $a^c = b$
- $4^2=x$

### Write as an exponential expression: $\log_2(64)=3x$

- $\log_a(b) = c$ is equivalent to $a^c = b$
- $2^{3x}=64$

### Write as an exponential expression: $\log_5(125)=2(2x-1)$

- $\log_a(b) = c$ is equivalent to $a^c = b$
- $5^{2(2x-1)}=125$
- $5^{4x-2}=125$

### Write as an exponential expression: $\log_y(27)=3$

- $\log_a(b) = c$ is equivalent to $a^c = b$
- $y^3=27$

### Write as an exponential expression: $\log_3(9)=x+1$

- $\log_a(b) = c$ is equivalent to $a^c = b$
- $3^{x+1}=9$

### Write as an exponential expression: $\log_{0.5}(0.125)=x-2$

- $\log_a(b) = c$ is equivalent to $a^c = b$
- $(0.5)^{x-2}=0.125$

### Write as an exponential expression: $\log_{x}(y)=z$

- $\log_a(b) = c$ is equivalent to $a^c = b$
- $x^z=y$

### Write as an exponential expression: $\log_{3x}(\frac{y-4}2)=z+1$

- $\log_a(b) = c$ is equivalent to $a^c = b$
- $(3x)^{z+1}=\frac{y-4}2$

