---
title: Cubic roots and coefficients
---

The roots in polynomials are closely linked to the coefficients of that
polynomial.

All polynomials in this chapter will be written as follows - the letters *are*
important here:

$$
ax^3+bx^2+cx+d
$$

## Sum of roots

If $p$, $q$ and $r$ are roots of $ax^3+bx^2+cx+d=0$, then $p+q+r=-\frac ba$.

This means that the *sum of roots* of a cubic is equal to $-\frac ba$.

### Find the sum of the roots of $x^3-6x^2+11x-6=0$

- The sum of roots is $-\frac ba$:
- $=-\frac{-6}1$
- $=6$
- **Answer**: sum of roots = $6$

### Find the sum of the roots of $2x^3+3x^2-4x+5=0$

- The sum of roots is $-\frac ba$:
- $=-\frac32$
- **Answer**: sum of roots = $-\frac32$

### The sum of the roots of the polynomial $x^3+kx^2+4x-8=0$ is 2. Find the value of $k$.

- Sum of roots = $2$ which represents $-\frac ba$.
- $2=-\frac k1$
- $k=-2$
- **Answer**: $k=-2$

### The sum of the roots of the polynomial $3x^3+mx^2-9x+12=0$ is -4. Find the value of $m$.

- Sum of roots = $-4$ which represents $-\frac ba$.
- $-4=-\frac m3$
- $m=12$
- **Answer**: $m=12$

## Sum of products of roots taken two at a time (sum of product 'pairs')

If $p$, $q$ and $r$ are roots of $ax^3+bx^2+cx+d=0$, then $pq+pr+qr=\frac ca$.

In other words, if we multiply together each possible pair of roots and then add
those products, we get the same result as $\frac ca$.

### Find the sum of product pairs for $x^3-6x^2+11x-6=0$

- The sum of product pairs is $\frac ca$:
- $=\frac{11}1$
- $=11$
- **Answer**: sum of product pairs = $11$

### Find the sum of product pairs for $2x^3+3x^2-4x+5=0$

- The sum of product pairs is $\frac ca$:
- $=\frac{-4}2$
- $=-2$
- **Answer**: sum of product pairs = $-2$

> The actual roots of this polynomial (+ some others here) are complex numbers.
> This shows us that actually, the answer above isn't really an answer! If we
> found the *actual* roots and found the sum of their product pairs, we wouldn't
> get a real number.

## Product of roots

If $p$, $q$ and $r$ are roots of $ax^3+bx^2+cx+d=0$, then
$p\times q\times r=-\frac da$.

In words, the *product of roots* of a cubic is equal to $-\frac da$.

### Find the product of the roots of $x^3-6x^2+11x-6=0$

- The product of roots is $-\frac da$:
- $=-\frac{-6}1$
- $=6$
- **Answer**: product of roots = $6$

### Find the product of the roots of $x^3-3x^2+3x-1=0$

- The product of roots is $-\frac da$:
- $=-\frac{-1}1$
- $=1$
- **Answer**: product of roots = $1$

### The equation $x^3+4x^2-x+2k=0$ has product of roots $6$. Find the value of $k$.

- The product of roots is $6$, which represents $-\frac da$.
- $6=-\frac{2k}1$
- $2k=-6$
- $k=-3$
- **Answer**: $k=-3$

### The equation $x^3-3x^2+4x+7=0$ has roots $p$, $q$ and $r$. Find the value of $\frac1p+\frac1q+\frac1r$.

- $\frac1p+\frac1q+\frac1r$
  - $=\frac{pq}{pqr}+\frac{pr}{pqr}+\frac{qr}{pqr}$
  - $=\frac{pq+pr+qr}{pqr}$
- Sum of product pairs = $\frac ca$:
  - $=\frac41=4$
  - So $pq+pr+qr=4$.
- Product of roots = $-\frac da$:
  - $=-\frac71=-7$
  - So $pqr=-7$.
- Therefore, $\frac1p+\frac1q+\frac1r$
  - $=\frac{pq+pr+qr}{pqr}$
  - $=\frac4{-7}$
  - $=-\frac47$
- **Answer**: $\frac1p+\frac1q+\frac1r=-\frac47$

## Summary of finding roots and coefficients

|                       | Coefficient link | Positive/Negative |
|-----------------------|------------------|-------------------|
| Sum of roots          | $-\frac ba$      | Negative          |
| Sum of products pairs | $\frac ca$       | Positive          |
| Product of roots      | $-\frac da$      | Negative          |

