---
title: Difference of two squares
---

Whenever we have an expression in the form of:

$$
a^2 - b^2
$$

We can factorise it into:

$$
(a - b)(a + b)
$$

Similarly, if we have an expression in the form of:

$$
(a - b)(a + b)
$$

We can expand it into:

$$
a^2 - b^2
$$

This has a lot of uses. For example, it's a key step in the method of
[rationalising the denominator](/rationalising-the-denominator) of a fraction.

## Examples

### Example: Factorise $x^2 - 9$

- We know that $a^2 - b^2$ factorises to $(a - b)(a + b)$.
- Here, $a = x$ and $b = 3$ (since $3^2 = 9$).
- So, $x^2 - 9$ factorises to $(x - 3)(x + 3)$.

**Answer**: $(x - 3)(x + 3)$

### Example: Expand $(x - 5)(x + 5)$

- We know that $(a - b)(a + b)$ expands to $a^2 - b^2$.
- Here, $a = x$ and $b = 5$.
- So, $(x - 5)(x + 5)$ expands to $x^2 - 25$.

**Answer**: $x^2 - 25$

### Example: Factorise $4x^2 - 1$

- We know that $a^2 - b^2$ factorises to $(a - b)(a + b)$.
- Here, $a = 2x$ (since $(2x)^2 = 4x^2$) and $b = 1$ (since $1^2 = 1$).
- So, $4x^2 - 1$ factorises to $(2x - 1)(2x + 1)$.

**Answer**: $(2x - 1)(2x + 1)$

