---
title: Distance between two points
---

To find the distance between two points (in a 2D plane) we can use the 
pythagorean theorem:

$$
a^2 + b^2 = c^2
$$

## Formula for distance between two points

We can derive this, however, by considering $a$ to be the difference in the
$x$-coordinates of the two points, $b$ to be the difference in the
$y$-coordinates of the two points, and $c$ to be the distance between the
two points:

$$
(x_2 - x_1)^2 + (y_2 - y_1)^2 = d^2
$$

Rearranging this to make $d$ the subject gives us the formula for the distance
between two points:

$$
d = \sqrt{(x_2 - x_1)^2 + (y_2 - y_1)^2}
$$

### Find the distance between the points (3, 4) and (7, 1).

- Values we know:
  - $x_1 = 3$
  - $y_1 = 4$
  - $x_2 = 7$
  - $y_2 = 1$
- Substitute into the formula:
  - $d = \sqrt{(x_2 - x_1)^2 + (y_2 - y_1)^2}$
  - $d = \sqrt{(7 - 3)^2 + (1 - 4)^2}$
  - $= \sqrt{(4)^2 + (-3)^2}$
  - $= \sqrt{16 + 9}$
  - $= \sqrt{25}$
  - $= 5$
- **Answer**: The distance between the points (3, 4) and (7, 1) is 5 units.

### Find the distance between the points (-2, 5) and (4, -1).

- Values we know:
  - $x_1 = -2$
  - $y_1 = 5$
  - $x_2 = 4$
  - $y_2 = -1$
- Substitute into the formula:
  - $d = \sqrt{(x_2 - x_1)^2 + (y_2 - y_1)^2}$
  - $d = \sqrt{(4 - (-2))^2 + (-1 - 5)^2}$
  - $= \sqrt{(6)^2 + (-6)^2}$
  - $= \sqrt{36 + 36}$
  - $= \sqrt{72}$
  - $= 6\sqrt{2}$
- **Answer**: The distance between the points (-2, 5) and (4, -1) is
  $6\sqrt{2}$ units.

