---
title: The factor theorem
---

The factor theorem states that:
> If $f(x)$ is a polynomial and $f(c) = 0$ for some constant $c$, then $(x - c)$
  is a factor of the polynomial $f(x)$.

This looks incredibly complicated, but you've already seen it before.

When you solve an equation that looks something like, for example,
$(x-2)(x+3)=0$, you used the factor theorem without even knowing it!

From that equation, you know that $2$ must be a root of the polynomial (in other
words, where $x=2$, the polynomial equals zero). You can also see that $(x-2)$
is a factor of the polynomial. This is exactly what the factor theorem states.

## Examples

### Find the two roots of the polynomial $f(x) = x^2 - x - 6$ using the factor theorem

- Factorise:
  - $(x-3)(x+2)$
- Find the roots:
  - If $(x-a)$ is a factor of the polynomial, then $f(a) = 0$.
  - We know that $(x-3)$ is a factor, so $f(3) = 0$.
  - We also know that $(x+2)$ is a factor, so $f(-2) = 0$.
- So the roots the roots of the polynomial are $x=3$ and $x=-2$.

### Given that $(x-3)$ is a factor of $f(x)$, find a root of $f(x)=0$

- The factor theorem states that if $(x-3)$ is a factor of $f(x)$, then
  $f(3)=0$.
- $f(3)=0$.
- $3$ is a root of $f(x)=0$.

## Other uses of the factor theorem

The factor theorem can also be used to help factorise polynomials which we
otherwise wouldn't know how to factorise.

For example, a cubic polynomial like $f(x) = x^3 - 6x^2 + 11x - 6$ is not
immediately factorable using simple methods. But if we know one of the roots,
we also know a factor, which then makes this much easier to factorise.

We cover that in the [polynomial division](polynomial-division) section.

