---
title: Finding the equation of a straight line
---

## Finding the equation of a straight line from two points

Let's suppose we know that two points are on a straight line - $(x, y)$ and
$(x_1, y_1)$ - and we want to find the equation of that straight line.

We need to know the **gradient** if we want to find the equation of the line,
and after that, we can substitute in our values for $x$, $y$, $x_1$, $y_1$ and
$m$ into the equation of a straight line: $y - y_1 = m(x - x_1)$.

### Finding the gradient

The gradient of a graph can be found by calculating the change in $y$ divided
by the change in $x$, or:

$$
m = \frac{\Delta y}{\Delta x}
$$

- The change in $y$ is going to be the *difference* between the starting $y$
  value - $y_1$ - and the ending $y$ value - $y$, so $\Delta y = y - y_1$.
- The change in $x$ is going to be the *difference* between the starting $x$
  value - $x_1$ - and the ending $x$ value - $x$, so $\Delta x = x - x_1$.

So, the gradient can be calculated using:

$$
m = \frac{y - y_1}{x - x_1}
$$

### Finding the equation of the line

Once you have found the gradient, you can substitute it into the equation of a
straight line:

$$
y - y_1 = m(x - x_1)
$$

### Example: find the equation of the straight line that passes through the points (2, 3) and (5, 11)

- Find the gradient:
  - $m = \frac{y - y_1}{x - x_1}$
  - $= \frac{11 - 3}{5 - 2}$
  - $= \frac{8}{3}$
- Substitute into the equation of a straight line:
  - $y - y_1 = m(x - x_1)$
  - $y - 3 = \frac{8}{3}(x - 2)$
- We can rearrange this into the form $y = mx + c$ *if we want to*:
  - $y - 3 = \frac{8}{3}x - \frac{16}{3}$
  - $y = \frac{8}{3}x - \frac{16}{3} + 3$
  - $y = \frac{8}{3}x - \frac{16}{3} + \frac{9}{3}$
  - $y = \frac{8}{3}x - \frac{7}{3}$
- **Answer**: $y = \frac{8}{3}x - \frac{7}{3}$

### Example: find the equation of the straight line that passes through the points (1, 4) and (3, 10)

- Find the gradient:
  - $m = \frac{y - y_1}{x - x_1}$
  - $= \frac{10 - 4}{3 - 1}$
  - $= \frac{6}{2}$
  - $= 3$
- Substitute into the equation of a straight line:
  - $y - y_1 = m(x - x_1)$
  - $y - 4 = 3(x - 1)$
- We can rearrange this into the form $y = mx + c$ *if we want to*:
  - $y - 4 = 3x - 3$
  - $y = 3x - 3 + 4$
  - $y = 3x + 1$
- **Answer**: $y = 3x + 1$

