---
title: Hyperbolic square difference identity
---

## $\cosh^2x - \sinh^2x = 1$

### Proof

- We know that:
  - $\sinh x = \frac{e^x - e^{-x}}{2}$
  - $\cosh x = \frac{e^x + e^{-x}}{2}$
- Square both functions:
  - $\sinh^2 x = \left(\frac{e^x - e^{-x}}{2}\right)^2 = \frac{e^{2x} - 2 + e^{-2x}}{4}$
  - $\cosh^2 x = \left(\frac{e^x + e^{-x}}{2}\right)^2 = \frac{e^{2x} + 2 + e^{-2x}}{4}$
- $\cosh^2 x - \sinh^2 x$
  - $= \frac{e^{2x} + 2 + e^{-2x}}{4} - \frac{e^{2x} - 2 + e^{-2x}}{4}$
  - $= \frac{e^{2x}+2+e^{-2x}-e^{2x}+2-e^{-2x}}4$
  - $= \frac44$
  - $=1$
- So we've shown that $\cosh^2x - \sinh^2x = 1$!

