---
title: Midpoint of points
---

The *midpoint* of two points is the point that is exactly halfway between them.

Importantly, this means that the $x$ and $y$ coordinates of the midpoint are the
*averages* of the $x$ and $y$ coordinates of the two points respectively.

## Finding the midpoint of two points

To find the midpoint of the two points, we can add up the x-coordinates of both
points, divide by 2 to get the average x-coordinate, and do the same for the
y-coordinates.

Or, use the formula:

$$
\text{Midpoint} = ( \frac{x_1 + x_2}{2}, \frac{y_1 + y_2}{2} )
$$

We can also separate the formula into its $x$ and $y$ components ($x_M$ and $y_M$ are the x and y coordinates of the midpoint respectively):

$$
x_M = \frac{x_1 + x_2}{2}
$$

$$
y_M = \frac{y_1 + y_2}{2}
$$

### Find the midpoint of the points (2, 3) and (6, 7).

- Values we know:
  - $x_1 = 2$
  - $y_1 = 3$
  - $x_2 = 6$
  - $y_2 = 7$
- Substitute into the formula:
  - $\text{Midpoint} = ( \frac{x_1 + x_2}{2}, \frac{y_1 + y_2}{2} )$
  - $= ( \frac{2 + 6}{2}, \frac{3 + 7}{2} )$
  - $= ( \frac{8}{2}, \frac{10}{2} )$
  - $= (4, 5)$
- **Answer**: (4, 5).

### Find the midpoint of the points (-1, 4) and (3, -2).

- Values we know:
  - $x_1 = -1$
  - $y_1 = 4$
  - $x_2 = 3$
  - $y_2 = -2$
- Substitute into the formula:
  - $\text{Midpoint} = ( \frac{x_1 + x_2}{2}, \frac{y_1 + y_2}{2} )$
  - $= ( \frac{-1 + 3}{2}, \frac{4 + (-2)}{2} )$
  - $= ( \frac{2}{2}, \frac{2}{2} )$
  - $= (1, 1)$
- **Answer**: (1, 1).

### Find the midpoint of the points (0, 0) and (5, 10).

- Values we know:
  - $x_1 = 0$
  - $y_1 = 0$
  - $x_2 = 5$
  - $y_2 = 10$
- Substitute into the formula:
  - $\text{Midpoint} = ( \frac{x_1 + x_2}{2}, \frac{y_1 + y_2}{2} )$
  - $= ( \frac{0 + 5}{2}, \frac{0 + 10}{2} )$
  - $= ( \frac{5}{2}, \frac{10}{2} )$
  - $= (2.5, 5)$
- **Answer**: (2.5, 5).

### Find the midpoint of the points (-4, -6) and (4, 6).

- Values we know:
  - $x_1 = -4$
  - $y_1 = -6$
  - $x_2 = 4$
  - $y_2 = 6$
- Substitute into the formula:
  - $\text{Midpoint} = ( \frac{x_1 + x_2}{2}, \frac{y_1 + y_2}{2} )$
  - $= ( \frac{-4 + 4}{2}, \frac{-6 + 6}{2} )$
  - $= ( \frac{0}{2}, \frac{0}{2} )$
  - $= (0, 0)$
- **Answer**: (0, 0).

## Finding one point given the other point and the midpoint

### Find the point A, given that the midpoint between point A and point B (4, 8) is (6, 10).

- Values we know:
  - Midpoint $= (6, 10)$
  - $x_2 = 4$
  - $y_2 = 8$
- Using the midpoint formula, we can set up two equations:
  - $6 = \frac{x_1 + 4}{2}$
  - $10 = \frac{y_1 + 8}{2}$
- Solving for $x_1$:
  - $6 \times 2 = x_1 + 4$
  - $12 = x_1 + 4$
  - $x_1 = 12 - 4$
  - $x_1 = 8$
- Solving for $y_1$:
  - $10 \times 2 = y_1 + 8$
  - $20 = y_1 + 8$
  - $y_1 = 20 - 8$
  - $y_1 = 12$
- **Answer**: Point A is (8, 12).

### Find the point C, given that the midpoint between point C and point D (2, -4) is (5, 1).

- Values we know:
  - Midpoint $= (5, 1)$
  - $x_2 = 2$
  - $y_2 = -4$
- Using the midpoint formula, we can set up two equations:
  - $5 = \frac{x_1 + 2}{2}$
  - $1 = \frac{y_1 + (-4)}{2}$
- Solving for $x_1$:
  - $5 \times 2 = x_1 + 2$
  - $10 = x_1 + 2$
  - $x_1 = 10 - 2$
  - $x_1 = 8$
- Solving for $y_1$:
  - $1 \times 2 = y_1 - 4$
  - $2 = y_1 - 4$
  - $y_1 = 2 + 4$
  - $y_1 = 6$
- **Answer**: Point C is (8, 6).

