---
title: Relationship of roots and coefficients of a quadratic
---

The roots in polynomials are closely linked to the coefficients of that
polynomial.

All polynomials in this chapter will be written as follows - the letters *are*
important here:

$$
ax^2+bx+c
$$

## Sum of roots

If $p$ and $q$ are roots of $ax^2+bx+c=0$, then $p+q=-\frac ba$.

This means that the *sum of roots* of a quadratic is equal to $-\frac ba$.

### Find the sum of the roots of $2x^2-5x+3=0$

- The sum of roots is $-\frac ba$:
- $=-\frac{-5}2$
- $=\frac52$
- **Answer**: sum of roots = $\frac52$

### Find the sum of the roots of $x^2+4x+4=0$

- The sum of roots is $-\frac ba$:
- $=-\frac41$
- $=-4$
- **Answer**: sum of roots = $-4$

### The sum of roots of the polynomial $3x^2+kx-9=0$ is 7. Find the value of $k$.

- $a=3$, $b=k$, $c=-9$
- The sum of roots is 7, which represents $-\frac ba$:
  - $7=-\frac k3$
  - $k=-21$
- **Answer**: $k=-21$

### The sum of roots of the polynomial $2x^2+2mx+3=0$ is -3. Find the value of $m$.

- $a=2$, $b=2m$, $c=3$
- The sum of roots is -3, which represents $-\frac ba$:
  - $-3=-\frac{2m}2$
  - $-3=-m$
  - $m=3$
- **Answer**: $m=3$

## Product of roots

If $p$ and $q$ are roots of $ax^2+bx+c=0$, then $p\times q=\frac ca$ (positive).

In words, the *product of roots* of a quadratic is equal to $\frac ca$.

### Find the product of the roots of $2x^2-5x+3=0$

- The product of roots is $\frac ca$:
- $=\frac32$
- **Answer**: product of roots = $\frac32$

### Find the product of the roots of $x^2+4x+4=0$

- The product of roots is $\frac ca$:
- $=\frac44$
- $=1$
- **Answer**: product of roots = $1$

### The product of roots of the polynomial $kx^2+10x+4$ is $\frac23$. Find the value of $k$.

- $a=k$, $b=10$, $c=4$
- The product of roots is $\frac23$, which represents $\frac ca$:
  - $\frac23=\frac4k$
  - $2k=12$
  - $k=6$
- **Answer**: $k=6$

## Evaluating other expressions

### The equation $x^2+5x+4=0$ has roots $p$ and $q$. Evaluate $p^2+q^2$

- The **only** things we know about $p$ and $q$ are:
  - $p+q=-\frac ba=-5$
  - $pq=\frac ca=4$
- We need to rewrite $p^2+q^2$ in terms of $p+q$ and $pq$ **only**:
  - $p^2+q^2=(p+q)^2-2pq$
- Now we can substitute the values we know in!
  - $=(-5)^2-2(4)$
  - $=25-8$
  - $=17$
- **Answer**: $p^2+q^2=17$

## Summary of finding roots and coefficients

|                     | Coefficient link | Positive/Negative |
|---------------------|------------------|-------------------|
| Sum of roots        | $-\frac ba$      | Negative          |
| Product of roots    | $\frac ca$       | Positive          |

