---
title: Quadratic formula
---

$$
x = \frac{-b \pm \sqrt{b^2 - 4ac}}{2a}
$$

## Uses of the quadratic formula

The main use is for solving the *roots* of a quadratic equation (finding the
values of $x$ where $y=0$)

It also has another use - the *discriminant* (the part under the square root)
can tell us a lot, for example, the number of roots the equation has. See
[the page on the discriminant](/discriminant) for more information.

## Finding the roots

To find the roots of a quadratic equation using the quadratic formula, we
substitute the coefficients of the equation into the quadratic formula.

The equation should be in the form $ax^2 + bx + c = 0$, so just substitute those
values into the formula above.

Remember to find both the positive and negative square roots of the discriminant
($b^2 - 4ac$) to get both roots! You can do this on your calculator by
calculating $+\sqrt{b^2 - 4ac}$ and $-\sqrt{b^2 - 4ac}$ separately.

## Example questions

### Find the roots of $2x^2 + 4x - 6 = 0$

- $a=2$
- $b=4$
- $c=-6$
- Substitute into the quadratic formula:
  - $x = \frac{-4 \pm \sqrt{4^2 - 4 \times 2 \times -6}}{2 \times 2}$
  - $x = \frac{-4 \pm \sqrt{16 + 48}}{4}$
  - $x = \frac{-4 \pm \sqrt{64}}{4}$
- Calculate both roots:
  - $x = \frac{-4 + 8}{4} = 1$
  - $x = \frac{-4 - 8}{4} = -3$
- **Answer**: $x = 1$ and $x = -3$

### Find the roots of $x^2 - 3x + 2 = 0$

- $a=1$
- $b=-3$
- $c=2$
- Substitute into the quadratic formula:
  - $x = \frac{-(-3) \pm \sqrt{(-3)^2 - 4 \times 1 \times 2}}{2 \times 1}$
  - $x = \frac{3 \pm \sqrt{9 - 8}}{2}$
  - $x = \frac{3 \pm \sqrt{1}}{2}$
- Calculate both roots:
  - $x = \frac{3 + 1}{2} = 2$
  - $x = \frac{3 - 1}{2} = 1$
- **Answer**: $x = 2$ and $x = 1$

### Find the roots of $3x^2 + 2x - 8 = 0$

- $a=3$
- $b=2$
- $c=-8$
- Substitute into the quadratic formula:
  - $x = \frac{-2 \pm \sqrt{2^2 - 4 \times 3 \times -8}}{2 \times 3}$
  - $x = \frac{-2 \pm \sqrt{4 + 96}}{6}$
  - $x = \frac{-2 \pm \sqrt{100}}{6}$
- Calculate both roots:
  - $x = \frac{-2 + 10}{6} = \frac{8}{6} = \frac{4}{3}$
  - $x = \frac{-2 - 10}{6} = \frac{-12}{6} = -2$
- **Answer**: $x = \frac{4}{3}$ and $x = -2$

