---
title: Raising an index to an index
---

When we have a number, and we raise it to a power, then raise the result to the
power of another number, we **multiply** the powers. This is much more easily
shown using algebra:

$$
(a^x)^y=a^{xy}
$$

> Note: if $a^x$ above is **not** surrounded with brackets, then this does not
> work, as it is then the power itself that is being raised to the second power.

### Example: simplify $(a^4)^7$

- $=a^{4\times7}$
- $=a^{28}$

### Example: simplify $(x^3)^2$

- $=x^{3\times2}$
- $=x^6$

### Example: evaluate $(2^3)^4$

- $=2^{3\times4}$
- $=2^{12}$
- $=4096$

### Example: evaluate $(2^4)^2$

- $=2^{4\times2}$
- $=2^8$
- $=256$

