---
title: Rationalising the denominator
---

## Rationalising the denominator

When we have a surd in the denominator of a fraction, we can **rationalise** the
denominator by multiplying both the numerator and denominator by the surd (or
the negated factor).

### Example: rationalise $\frac{1}{\sqrt{2}}$

- $=\frac{1\times\sqrt{2}}{\sqrt{2}\times\sqrt{2}}$
- $=\frac{\sqrt{2}}{2}$

### Example: rationalise $\frac{3}{\sqrt{5}}$

- $=\frac{3\times\sqrt{5}}{\sqrt{5}\times\sqrt{5}}$
- $=\frac{3\sqrt{5}}{5}$

### Example: rationalise $\frac{4}{\sqrt{3}}$

- $=\frac{4\times\sqrt{3}}{\sqrt{3}\times\sqrt{3}}$
- $=\frac{4\sqrt{3}}{3}$

### Example: rationalise $\frac{\sqrt{2}}{1+\sqrt{3}}$

- $=\frac{\sqrt{2}(1-\sqrt{3})}{(1+\sqrt{3})(1-\sqrt{3})}$
- $=\frac{\sqrt{2}-\sqrt{6}}{1-3}$
- $=\frac{\sqrt{2}-\sqrt{6}}{-2}$

### Example: rationalise $\frac{5}{2+\sqrt{7}}$

- $=\frac{5(2-\sqrt{7})}{(2+\sqrt{7})(2-\sqrt{7})}$
- $=\frac{10-5\sqrt{7}}{4-7}$
- $=\frac{10-5\sqrt{7}}{-3}$

### Example: rationalise $\frac{3\sqrt{5}}{4-\sqrt{2}}$

- $=\frac{3\sqrt{5}(4+\sqrt{2})}{(4-\sqrt{2})(4+\sqrt{2})}$
- $=\frac{12\sqrt{5}+3\sqrt{10}}{16-2}$
- $=\frac{12\sqrt{5}+3\sqrt{10}}{14}$

