---
title: Subtracting logarithms
---

When subtracting logarithms with the same base, it's equivalent to dividing
the values inside the logarithms:

$$
\log_b(x) - \log_b(y) = \log_b\left(\frac{x}{y}\right)
$$

## Subtracting two logarithms

### Example: Evaluate $\log_4(64) - \log_4(16)$

- Both have the same base of 4.
- Divide the values inside: $\frac{64}{16} = 4$.
- So, $\log_4(64) - \log_4(16) = \log_4(4)$.
- $\log_4(4)=1$ because $4^1=4$.
- **Answer:** $1$.

### Example: Evaluate $\log_{10}(10000) - \log_{10}(100)$

- Both have the same base of 10.
- Divide the values inside: $\frac{10000}{100} = 100$.
- So, $\log_{10}(10000) - \log_{10}(100) = \log_{10}(100)$.
- $\log_{10}(100)=2$ because $10^2=100$.
- **Answer:** $2$.

## Subtracting more than two logarithms

We can do exactly the same when we are subtracting more than two logarithms with
the same base - just divide all the values inside.

### Example: Evaluate $\log_2(256) - \log_2(16) - \log_2(4)$

- All have the same base of 2.
- Divide the values inside: $\frac{256}{16 \times 4} = \1$.
- So, $\log_2(256) - \log_2(16) - \log_2(4) = \log_2(1)$.
- $\log_2(1)=0$ because $2^0=1$.
- **Answer:** $0$.

## Splitting up a logarithm with subtraction

You can also split up a logarithm into the difference of two logarithms:

$$
\log_b\left(\frac{x}{y}\right) = \log_b(x) - \log_b(y)
$$

This isn't usually needed, but it's good to know it works both ways (is
*bidirectional*).

